\documentclass[a4paper]{article}

\usepackage{amssymb}
\usepackage{euscript}
\usepackage{graphicx}
\graphicspath{{pics/}}
\usepackage{color}
\usepackage{epsfig}

\begin{document}

\subsection*{Gradient energy}

\hrule

\begin{eqnarray*}
F_\nabla
&=& \frac12 K_1 (\nabla_j d_{\mu k})(\nabla_j d^*_{\mu k})\\
&+& \frac12 K_2 (\nabla_j d_{\mu k})(\nabla_k d^*_{\mu j})\\
&+& \frac12 K_3 (\nabla_j d_{\mu j})(\nabla_k d^*_{\mu k})
\qquad{\rm\small (VW 7.17)}\\
\end{eqnarray*}

B-phase, no distorsion of order parameter ("London limit"),
{\it bending energy}:

$$
d_{\mu j}=\Delta R_{\mu j} e^{i\phi},\qquad
R_{\mu j} R_{\mu k} = \delta_{jk}
$$

\begin{eqnarray*}
F_\nabla
&=& \frac12 \Delta^2 K_1
 (\nabla_j R_{\mu k})(\nabla_j R_{\mu k})\\
&+& \frac12 \Delta^2 K_2
 (\nabla_j R_{\mu k})(\nabla_k R_{\mu j})\\
&+& \frac12 \Delta^2 K_3
 (\nabla_j R_{\mu j})(\nabla_k R_{\mu k})\\
&+& \frac12 \Delta^2 (3K_1+K_2+K_3)
 (\nabla_j \phi)(\nabla_j \phi)\\
\end{eqnarray*}

Terms with $K_2$ and $K_3$:
$$
(\nabla_j R_{\mu k})(\nabla_k R_{\mu j}) - (\nabla_j R_{\mu j})(\nabla_k R_{\mu k}) =
\nabla_k(R_{\mu j} \nabla_j R_{\mu k} - R_{\mu k} \nabla_j R_{\mu j}) =
2\nabla_k(R_{\mu j} \nabla_j R_{\mu k})
$$
\begin{eqnarray*}
F_\nabla
&=& \frac12\Delta^2 K_1 (\nabla_j R_{\mu k})(\nabla_j R_{\mu k})\\
&+& \frac12\Delta^2 (K_2+K_3) (\nabla_j R_{\mu j})(\nabla_k R_{\mu k})\\
&+& \Delta^2 K_2 \nabla_k(R_{\mu j} \nabla_j R_{\mu k}),\qquad
\rightarrow \mbox{surface term}\\
&+& \frac12 \Delta^2 (3K_1+K_2+K_3)
 (\nabla_j \phi)(\nabla_j \phi)\\
\end{eqnarray*}

Relation between $K_{1,2,3}$ and Thuneberg's $\lambda_{G1,G2}$
$$
\lambda_{G1} = \frac12\Delta^2 (K_2+K_3),\qquad
\lambda_{G2} = \frac12\Delta^2 K_1,\qquad
\lambda_{SG}^b = \Delta^2 K_2
$$

Without Fermi-liquid corrections (VW 7.23m):

$$
K_1=K_2=K_3 = \frac{1}{5\Delta^2} \left(\frac{h}{2m}\right)^2 (1-Y_0)\rho
$$

\eject

%%%%%%%%%%%%%%%%%%%%%%%%%%%%%%%%%%%%%%%%%%%%%%%%%%%%%%%%%%%%%%%%%%%%%%
\hrule
\medskip

Small rotation $\theta^{so}_j$ (VW 7.25):

$$
R_{\alpha\j} = R_{jk}(\theta^{so}) R^0_{\alpha k} =
(\delta_{jk} - e_{jkn}\theta^{so}_n) R^0_{\alpha k}
$$

\begin{eqnarray*}
F_\nabla
&=& \frac12 \Delta^2\ (2 K_1 + K_2 + K_3)
\nabla_j\theta^{so}_k \nabla_j\theta^{so}_k\\
&-& \frac12 \Delta^2\ K_2
\nabla_j\theta^{so}_j \nabla_k\theta^{so}_k\\
&-& \frac12 \Delta^2\ K_3
\nabla_j\theta^{so}_k \nabla_k\theta^{so}_j\\
\end{eqnarray*}

math:
$$
\nabla_j \theta_k \nabla_k \theta_j = (\nabla \cdot \theta)^2 +
\nabla_k(\theta_j \nabla_j\theta_k - \theta_k \nabla_j\theta_j)
$$
$$
 \nabla_j \theta_k \nabla_j \theta_k = [\nabla \times \theta]^2 + \nabla_j \theta_k \nabla_k \theta_j
$$

\begin{eqnarray*}
F_\nabla
&=& \frac12 \Delta^2\ (2 K_1 + K_2 + K_3)
[\nabla \times \theta^{so}]^2\\
&+& \frac12 \Delta^2\  2K_1
(\nabla \cdot \theta^{so})^2\\
&+& \frac12 \Delta^2\ (2 K_1+K_2)
\nabla_k(\theta^{so}_j \nabla_j\theta^{so}_k - \theta^{so}_k \nabla_j\theta^{so}_j)\\
\end{eqnarray*}

Weak couplng:
$$
2 K_1 + K_2 + K_3 = \frac{2}{\Delta^2}\left(\frac{\hbar}{2m}\right)^2 a,
\qquad
K_2 = -\frac{2}{\Delta^2}\left(\frac{\hbar}{2m}\right)^2 c,
\qquad
K_3 = -\frac{2}{\Delta^2}\left(\frac{\hbar}{2m}\right)^2 b
$$
$$
a=-(4+\delta)c,\qquad
b= (1+\delta)c,\qquad
c=-\frac{\rho_s}{10}
\ \frac{3+F_1^a}{3+F_1^s}
\ \frac{1}{1+F_1^a(5-3\rho_s/\rho)/15}
,\qquad
\delta = \frac{F_1^a \rho_s/\rho}{3+F_1^s(1-\rho_s/\rho)}
$$

$$
K_2+K_3 = (2+\delta)K_2,\qquad
K_1=K_2,\qquad
$$
$$
\lambda_{G1} = \frac{\Delta^2}{2}(K_2+K3) = -\left(\frac{\hbar}{2m}\right)^2 (2+\delta) c,\qquad
\lambda_{G2} = \frac{\Delta^2}{2}K_1 = -\left(\frac{\hbar}{2m}\right)^2 c,\qquad
\lambda_{SG}^B = 2\lambda_{G2}
$$

$$
F_\nabla = \lambda_{G2} \left[
   (4+\delta) [\nabla \times \theta^{so}]^2
  + 2 (\nabla \cdot \theta^{so})^2
  + 3 \nabla_k(\theta^{so}_j \nabla_j\theta^{so}_k - \theta^{so}_k \nabla_j\theta^{so}_j)
\right]
$$

\eject
%%%%%%%%%%%%%%%%%%%%%%%%%%%%%%%%%%%%%%%%%%%%%%%%%%%%%%%%%%%%%%%%%%%%%%
\hrule
\medskip

Small rotation $\theta^s_\alpha$ (VW 8.157-160):

$$
R_{\alpha i} = R_{\alpha\beta}(\theta^s) R^0_{\beta i} =
(\delta_{\alpha\beta} - e_{\alpha\beta \gamma}\theta^s_\gamma) R^0_{\beta i},
\qquad
\nabla_j R_{\alpha i} = 
- e_{\alpha\beta \gamma}\nabla_j \theta^s_\gamma R^0_{\beta i}.
$$

Fomin's notation $\omega_{\gamma j} = \nabla_j \theta^s_\gamma$.

\begin{eqnarray*}
F_\nabla
&=& \frac12 \Delta^2\ (2 K_1 + K_2 + K_3)
(\nabla_i\theta^s_\alpha) (\nabla_i\theta^s_\alpha)\\
&-& \frac12 \Delta^2\  K_2
\ R^0_{\alpha i}R^0_{\beta j}(\nabla_i\theta^s_\alpha)(\nabla_j\theta^s_\beta)\\
&-& \frac12 \Delta^2\ K_3
\ R^0_{\alpha i}R^0_{\beta j}(\nabla_i\theta^s_\beta) (\nabla_j\theta^s_\alpha)\\
\end{eqnarray*}

math:
$$
\nabla_i(\theta_\alpha \nabla_j\theta_\beta - \theta_\beta \nabla_j\theta_\alpha) =
(\nabla_i\theta_\alpha)(\nabla_j\theta_\beta) -(\nabla_i\theta_\beta) (\nabla_j\theta_\alpha)
+ \theta_\alpha \nabla_i\nabla_j\theta_\beta - \theta_\beta \nabla_i\nabla_j\theta_\alpha
$$

\begin{eqnarray*}
F_\nabla
&=& \frac12 \Delta^2\ (2 K_1 + K_2 + K_3)
(\nabla_i\theta^s_\alpha) (\nabla_i\theta^s_\alpha)\\
&-& \frac12 \Delta^2\ (K_2+K_3)
R^0_{\alpha i}R^0_{\beta j}(\nabla_i\theta^s_\alpha)(\nabla_j\theta^s_\beta)\\
&+& \frac12 \Delta^2\ K_3
\ R^0_{\alpha i}R^0_{\beta j}
\ \nabla_i(\theta^s_\alpha \nabla_j\theta^s_\beta - \theta^s_\beta \nabla_j\theta^s_\alpha)\\
\end{eqnarray*}
$$
K=2K_1+K_2+K_3,\qquad K'=K_2+K_3
$$

Fomin's spin wave velocities (see Fomin-1980 f.51):

$$
\frac12\Delta^2 K  = \frac{\chi}{2\gamma^2} c_\parallel^2,\qquad
\frac12\Delta^2 K' = 2\ \frac{\chi}{2\gamma^2} (c_\parallel^2 - c_\perp^2).
$$

$$
c_\parallel^2 = \frac{\gamma^2 \Delta^2}{\chi} K,\qquad
c_\perp^2 = \frac{\gamma^2 \Delta^2}{\chi} (K-K'/2)
$$

in terms of $\lambda_{G2}$ and $\delta$ in weak coupling approximation:

$$
c_\parallel^2 = \frac{2\gamma^2}{\chi} (4+\delta)\lambda_{G2},\qquad
c_\perp^2     = \frac{2\gamma^2}{\chi} (3+\delta/2)\lambda_{G2}
$$

%%%%%%%%%%%%%%%%%%%%%%%%%%%%%%%%%%%%%%%%%%%%%%%%%%%%%%%%%%%%%%%%%%%%%%
\hrule
\medskip

Shrodinger equations for magnons (VW 8.179).

$$
-(\bar K - \bar K'/2)\xi_D^2 \Delta\Psi - (1- \frac12 \sin^2\beta_N) \Psi = E \Psi.
$$

$$
\xi_D^2 (\bar K- \bar K'/2) = \Delta^2 \gamma^2/\chi \Omega_B^2 (K-K'/2)
=\Omega_B^2 c_\perp^2
$$




\end{document}
